 \documentclass[12pt]{article}

\usepackage[margin=1in]{geometry}
\usepackage{fancyhdr}
\usepackage{setspace}
\pagestyle{fancy}
\usepackage{amsmath, amsthm, amssymb, amsfonts, mathtools, xfrac,mathrsfs}
\usepackage[utf8]{inputenc}
\usepackage[english]{babel}
\usepackage{graphicx,dsfont}
\usepackage{braket, bm}

\everymath{\displaystyle}
\headheight=20pt


\newcommand{\N}{\mathbb{N}}
\newcommand{\Z}{\mathbb{Z}}
\newcommand{\Q}{\mathbb{Q}}
\newcommand{\R}{\mathbb{R}}
\newcommand{\E}{\mathrm{E}}
\newcommand{\Var} {\mathrm{Var}}
\newcommand{\Cov}{\mathrm{Cov}}
\newcommand{\F}{\mathbb{F}}

\DeclareMathOperator{\Tr}{Tr}

\def\mean#1{\left< #1 \right>}
 
\newcommand*\rfrac[2]{{}^{#1}\!/_{#2}}
 
\newenvironment{theorem}[2][Theorem]{\begin{trivlist}
\item[\hskip \labelsep {\bfseries #1}\hskip \labelsep {\bfseries #2}]}{\end{trivlist}}

\newenvironment{problem}[2][Problem]{\begin{trivlist}
\item[\hskip \labelsep {\bfseries #1}\hskip \labelsep {\bfseries #2}]}{\end{trivlist}}

\title{Homework}
\lhead{Econ OSM Lab}
\chead{DSGE}
\rhead{Dan Ehrlich}
 
\begin{document}

\begin{problem}{1.} 
For the Brock and Mirman model, find the value of $A$ in the policy function by guessing a policy function $K_{t+1} = Ae^{zt}K_t^\alpha$ and plugging it into the Euler equation. We therefore have then that 
\begin{align*}
\frac{1}{ e^{z_t} K_t^\alpha - K_{t+1}} &= \beta E_t \big\{\frac{\alpha e^{z_{t+1}} K_{t+1}^{\alpha-1}}{e^{z_{t+1}}K_{t+1}^\alpha - K_{t+2}}\big\} \\
\frac{1}{ (1-A)e^{z_t} K_t^\alpha} &= \beta E_t \big\{\frac{\alpha e^{z_{t+1}} K_{t+1}^{\alpha-1}}{(1-A)e^{z_{t+1}}K_{t+1}^\alpha}\big\} \\
\frac{1}{ e^{z_t} K_t^\alpha} &= \beta \frac{\alpha}{K_{t+1}}\\
\frac{1}{ e^{z_t} K_t^\alpha} &= \beta \frac{\alpha}{Ae^{zt}K_t^\alpha}\\
1 &= \frac{\alpha \beta}{A}\\
A &= \alpha\beta
\end{align*}
\end{problem}

\begin{problem}{2.}
Given following functional forms,
\begin{equation}
\begin{split}
u(c_t,\ell_t) & = \text{ln }c_t + a \text{ ln }(1-\ell_t)\\
F(K_t,L_t,z_t) & = e^{z_t}K^{\alpha}_t L^{1-\alpha}_t  \nonumber
\end{split}
\end{equation}
there are 7 characterizing equations:
$$c_t = (1-\tau)(w_tl_t + (r_t -\delta)k_t) + k_t + T_t - k_{t+1}$$
$$\frac{1}{c_t} = \beta E_t \big\{ \frac{1}{c_{t+1}}((r_{t+1} - \delta)(1-\tau)+ 1) \big\}$$
$$\frac{a}{1-l_t} = \frac{w_t}{c_t}(1-\tau)$$
$$r_t = \alpha e^{zt}K_t^{\alpha-1} L_t^{1-\alpha}$$
$$w_t = (1-\alpha) e^{zt}K_t^{\alpha} L_t^{-\alpha}$$
$$\tau(w_tl_t + (r_t -\delta)k_t) = T_t$$
$$z_t = (1-p_z)\bar{z} + p_zz_{t-1} + \epsilon^z_t,  \epsilon^z_t \sim \text{i.i.d}(0, \sigma^2_z)$$
\end{problem}

\begin{problem}{3.}
Using the new given functional forms,
\begin{equation}\label{DSGE_HW_CharEq_CES_Ln_eq01}
\begin{split}
u(c_t,\ell_t) & = \frac{c^{1-\gamma}_t -1}{1-\gamma}+ a \text{ ln }(1-\ell_t)\\
F(K_t,L_t,z_t) & = e^{z_t}K^{\alpha}_t L^{1-\alpha}_t  \nonumber
\end{split}
\end{equation}
we can again solve for the 7 characterizing equations:
$$c_t = (1-\tau)(w_tl_t + (r_t -\delta)k_t) + k_t + T_t - k_{t+1}$$
$$\frac{1}{c_t^{-\gamma}} = \beta E_t \big\{ \frac{1}{c_{t+1}^{-\gamma}}((r_{t+1} - \delta)(1-\tau)+ 1) \big\}$$
$$\frac{a}{1-l_t} = \frac{w_t}{c_t^{-\gamma}}(1-\tau)$$
$$r_t = \alpha e^{zt}K_t^{\alpha-1} L_t^{1-\alpha}$$
$$w_t = (1-\alpha) e^{zt}K_t^{\alpha} L_t^{-\alpha}$$
$$\tau(w_tl_t + (r_t -\delta)k_t) = T_t$$
$$z_t = (1-p_z)\bar{z} + p_zz_{t-1} + \epsilon^z_t,  \epsilon^z_t \sim \text{i.i.d}(0, \sigma^2_z)$$
\end{problem}

\begin{problem}{4.} 
Using the new given function forms,
\begin{equation}\label{DSGE_HW_CharEq_CES_eq01}
\begin{split}
u(c_t,\ell_t) & = \frac{c^{1-\gamma}_t -1}{1-\gamma}+ a \frac{(1-\ell_t)^{1-\xi}-1}{1-\xi}      \\
F(K_t,L_t,z_t) & = e^{z_t}\left[\alpha K^{\eta}_t +(1-\alpha)L^{\eta}_t \right]^{\frac{1}{\eta}}   \nonumber
\end{split}
\end{equation}
we can again solve for the 7 characterizing equations:
$$c_t = (1-\tau)(w_tl_t + (r_t -\delta)k_t) + k_t + T_t - k_{t+1}$$
$$\frac{1}{c_t^{-\gamma}} = \beta E_t \big\{ \frac{1}{c_{t+1}^{-\gamma}}((r_{t+1} - \delta)(1-\tau)+ 1) \big\}$$
$$\frac{a}{(1-l_t)^{-\xi}} = \frac{w_t}{c_t^{-\gamma}}(1-\tau)$$
$$r_t = \alpha e^{zt}K_t^{\eta-1} (\alpha K_t^\eta+ (1-\alpha)L_t^\eta)^{\frac{1-\eta}{\eta}}$$
$$w_t = (1-\alpha) e^{zt}L_t^{\eta-1}(\alpha K_t^\eta+ (1-\alpha)L_t^\eta)^{\frac{1-\eta}{\eta}}$$
$$\tau(w_tl_t + (r_t -\delta)k_t) = T_t$$
$$z_t = (1-p_z)\bar{z} + p_zz_{t-1} + \epsilon^z_t,  \epsilon^z_t \sim \text{i.i.d}(0, \sigma^2_z)$$
\end{problem}

\begin{problem}{5.} 
Using the new given functional forms.
\begin{equation}\label{DSGE_HW_NoLeisure_eq01}
\begin{split}
u(c_t) & = \frac{c^{1-\gamma}_t -1}{1-\gamma}      \\
F(K_t,L_t,z_t) & = K^{\alpha}_t (L_te^{z_t})^{1-\alpha}  \nonumber
\end{split}
\end{equation}
we can again solve for the 6 characterizing equations: 
$$c_t = (1-\tau)(w_t+ (r_t -\delta)k_t) + k_t + T_t - k_{t+1}$$
$$\frac{1}{c_t^{-\gamma}} = \beta E_t \big\{ \frac{1}{c_{t+1}^{-\gamma}}((r_{t+1} - \delta)(1-\tau)+ 1) \big\}$$
$$r_t = \alpha (e^{zt})^{(1-\alpha)} K_t^{\alpha-1} $$
$$w_t = (1-\alpha) (e^{zt})^{(1-\alpha)} K_t^{\alpha} $$
$$\tau(w_t + (r_t -\delta)k_t) = T_t$$
$$z_t = (1-p_z)\bar{z} + p_zz_{t-1} + \epsilon^z_t,  \epsilon^z_t \sim \text{i.i.d}(0, \sigma^2_z)$$
which in the steady state become:
$$\bar{c} = (1-\tau)(\bar{w} + (\bar{r} -\delta)\bar{k}) + \bar{T}$$
$$\frac{1}{\bar{c}^{-\gamma}} = \beta \frac{1}{\bar{c}^{-\gamma}}((\bar{r} - \delta)(1-\tau)+ 1) $$
$$\bar{r} = \alpha (e^{\bar{z}})^{1-\alpha} \bar{k}^{\alpha-1} $$
$$\bar{w} = (1-\alpha) (e^{\bar{z}})^{1-\alpha} \bar{k}^{\alpha} $$
$$\tau(\bar{w} + (\bar{r} -\delta)\bar{k}) =  \bar{T}$$
where $\bar{z} = 0$. Solving algebraically for the steady state values of capital, output, and investment, we have that:
$$\bar{r} = \frac{\frac{1}{\beta}-1}{1-\tau} + \delta = 0.12$$
$$\bar{k} = \big(\frac{\bar{r}}{\alpha}\big)^\frac{1}{\alpha-1} = 7.28$$
$$\bar{I} = \delta \bar{k} = 0.73$$
$$\bar{Y} = \bar{k}^\alpha = 2.21$$
For the numerical solution (which is equivalent to the algebraic), refer to the appropriate python notebook.
 \end{problem}
\begin{problem}{6.} 
Using the new given functional forms.
\begin{equation}\label{DSGE_HW_CES_eq01}
\begin{split}
u(c_t,\ell_t) & = \frac{c^{1-\gamma}_t -1}{1-\gamma}+ a \frac{(1-\ell_t)^{1-\xi}-1}{1-\xi}      \\
F(K_t,L_t,z_t) & = K^{\alpha}_t (L_te^{z_t})^{1-\alpha}  \nonumber
\end{split}
\end{equation}
we can again solve for the 7 characterizing equations: 
$$c_t = (1-\tau)(w_t+ (r_t -\delta)k_t) + k_t + T_t - k_{t+1}$$
$$\frac{1}{c_t^{-\gamma}} = \beta E_t \big\{ \frac{1}{c_{t+1}^{-\gamma}}((r_{t+1} - \delta)(1-\tau)+ 1) \big\}$$
$$\frac{a}{(1-l_t)^{-\xi}} = \frac{w_t}{c_t^{-\gamma}}(1-\tau)$$
$$r_t = \alpha (e^{zt})^{1-\alpha} K_t^{\alpha-1} L_t^ {1-\alpha}$$
$$w_t = (1-\alpha) (e^{zt})^{1-\alpha} K_t^{\alpha}L_t^ {-\alpha} $$
$$\tau(w_t + (r_t -\delta)k_t) = T_t$$
$$z_t = (1-p_z)\bar{z} + p_zz_{t-1} + \epsilon^z_t,  \epsilon^z_t \sim \text{i.i.d}(0, \sigma^2_z)$$
which in the steady state become:
$$\bar{c} = (1-\tau)(\bar{w} + (\bar{r} -\delta)\bar{k}) + \bar{T}$$
$$\frac{1}{\bar{c}^{-\gamma}} = \beta \frac{1}{\bar{c}^{-\gamma}}((\bar{r} - \delta)(1-\tau)+ 1) $$
$$\frac{a}{(1-\bar{l})^{-\xi}} = \frac{\bar{w}}{\bar{c}^{-\gamma}}(1-\tau)$$
$$\bar{r} = \alpha (e^{\bar{z}})^{1-\alpha} \bar{k}^{\alpha-1} \bar{l}^{1-\alpha} $$
$$\bar{w} = (1-\alpha) (e^{\bar{z}})^{1-\alpha} \bar{k}^{\alpha} \bar{l}^{-\alpha}$$
$$\tau(\bar{w} + (\bar{r} -\delta)\bar{k}) =  \bar{T}$$
where $\bar{z} = 0$. 
For the numerical solution (which is equivalent to the algebraic), refer to the appropriate python notebook.
\end{problem}

\begin{problem}{8.} 
Refer to the appropriate python notebook. 
\end{problem}

\end{document}

